improved compile_cont to parallel match

Test/tutorial/ImpVerifiedCompiler/Proof2.dfy
@@ -1,17 +1,5 @@
 include "Proof.dfy"
 
-predicate Star<T(!new)>(R: (T,T) -> bool, conf1: T, conf2: T) {
-  star(R, conf1, conf2)
-}
-
-least predicate Plus<T(!new)>(R: (T,T) -> bool, conf1: T, conf2: T) {
-	plus(R,conf1, conf2)
-}
-
-greatest predicate Inf<T(!new)>(R: (T,T) -> bool,conf: T) {
-	inf(R,conf)
-}
-
 least lemma simulation_steps(C: code, impconf1: conf, impconf2: conf, machconf1: configuration)
 	requires star(step,impconf1,impconf2)
 	requires match_config(C, impconf1, machconf1)
