Test/tutorial/ImpVerifiedCompiler/SimulationRelationCont.dfy
@@ -31,20 +31,20 @@ include "SemanticsProperties.dfy"
 
 least predicate compile_cont(C: code, k: cont, pc: nat) {
 	if ! (pc < |C|) then false else
-	 match (k,C[pc]) {
+	 (match (k,C[pc]) {
 		case (Kstop,Ihalt) => true
 		case _ => false
-	 }
+	 })
 	 ||
-		match (k,C[pc]) {
+		((match (k,C[pc]) {
 	 		case (Kseq(c,k),_) =>
 	 			var pc': nat := pc + |compile_com(c)|;
 	 			&& code_at(C, pc, (compile_com(c)))
 	 				&& compile_cont(C, k, pc')
 	 		case _ => false
-		}
+		})
 		||
-			match (k,C[pc]) {
+			((match (k,C[pc]) {
 				case (Kwhile(b,c,k),Ibranch(ofs)) =>
 					var pc' := pc + 1 + ofs;
 					var pc'' := pc' + |compile_com(CWhile(b, c))|;
@@ -53,15 +53,15 @@ least predicate compile_cont(C: code, k: cont, pc: nat) {
 						&& code_at(C, pc', (compile_com(CWhile(b, c)))) 
 						&& compile_cont(C, k, pc'')
 				case _ => false
-			}
+			})
 			||
-				match (k,C[pc]) {
+				(match (k,C[pc]) {
 					case (_,Ibranch(ofs)) =>
 						var pc' := pc + 1 + ofs;
 						&& pc' > 0
 							&& compile_cont(C, k, pc')
 					case _ => false
-				}
+				})))
 }
 
 predicate match_config(C: code, hl: conf, ll:configuration) {
@@ -106,35 +106,57 @@ least lemma compile_cont_Kstop_inv(C: code, pc: nat, s: store)
 		
 }
 
-lemma {:axiom} compile_cont_Kseq_inv(C: code, c: com, k: cont, pc: nat, s: store)
-	requires compile_cont(C,(Kseq(c,k)),pc)
+least lemma compile_cont_Kseq_inv(C: code, c: com, k: cont, pc: nat, s: store)
+	requires compile_cont(C,Kseq(c,k),pc)
 	ensures exists pc': nat :: star((c1,c2) => transition(C,c1,c2),(pc, [], s),(pc', [], s)) && code_at(C,pc',compile_com(c)) && compile_cont(C,k,pc' + |compile_com(c)|)
-//{
-//}
+{
+}
 
-lemma {:axiom} compile_cont_Kwhile_inv(C: code, b: bexp, c: com, k: cont, pc: nat, s: store)
-	requires compile_cont(C,(Kwhile(b,c,k)),pc)
+lemma compile_cont_Kwhile_simp(C: code, b: bexp, c: com, k: cont, pc: nat, s: store, ofs: int)
+	requires compile_cont(C,Kwhile(b,c,k),pc)
+	requires C[pc] == Ibranch(ofs)
+	ensures 
+	|| (pc + 1 + ofs > 0 && compile_cont(C, Kwhile(b,c,k), pc + 1 + ofs))
+	|| (&& pc + 1 + ofs > 0
+	   && (pc + 1 + ofs) + |compile_com(CWhile(b, c))| > 0
+ 		 && code_at(C, pc + 1 + ofs, (compile_com(CWhile(b, c))))
+ 		 && compile_cont(C, k, (pc + 1 + ofs) + |compile_com(CWhile(b, c))|))
+{
+}
+		 
+
+least lemma compile_cont_Kwhile_inv(C: code, b: bexp, c: com, k: cont, pc: nat, s: store)
+	requires compile_cont(C,Kwhile(b,c,k),pc)
 	ensures exists pc': nat :: plus((c1,c2) => transition(C,c1,c2),(pc, [], s),(pc', [], s)) && code_at(C,pc',compile_com(CWhile(b,c))) && compile_cont(C,k,pc' + |compile_com(CWhile(b,c))|)
-// {
+{
 
-// 	match C[pc] {
+	match C[pc] {
 
-// 		case Ibranch(ofs) => {
+		case Ibranch(ofs) => {
 
-// 			var pc': nat := pc + 1 + ofs;
-// 			var pc'': nat := pc' + |compile_com(CWhile(b, c))|;
-// 			assert pc' > 0;
-// 			assert pc'' > 0;	
-// 			assert code_at(C, pc', (compile_com(CWhile(b, c)))); 
-// 			assert compile_cont(C, k, pc'');
+			compile_cont_Kwhile_simp(C,b,c,k,pc,s,ofs);
 
-// 			assert transition(C,(pc, [], s),(pc', [], s));
-// 			plus_one<configuration>((c1,c2) => transition(C,c1,c2),(pc, [], s),(pc', [], s));
+			if pc + 1 + ofs > 0 && compile_cont(C, Kwhile(b,c,k), pc + 1 + ofs) {
+
+ 				var pc': nat := pc + 1 + ofs;
+
+				assert transition(C,(pc, [], s),(pc', [], s));
+ 				plus_one<configuration>((c1,c2) => transition(C,c1,c2),(pc, [], s),(pc', [], s));
+				
+				compile_cont_Kwhile_inv(C,b,c,k,pc',s);
+				
+ 			} else {
+
+				assert transition(C,(pc, [], s),(pc + 1 + ofs, [], s));
+ 				plus_one<configuration>((c1,c2) => transition(C,c1,c2),(pc, [], s),(pc + 1 + ofs, [], s));
+				
+			}
 			
-// 		}
-
-// 		case _ => 
+		}
 		
-// 	}
-	
-// }
+		case _ =>
+
+	}
+
+}
+
